SciLean/Core/Monad/FwdDiff/StateM.lean
@@ -1,32 +1,63 @@
-import SciLean.Core.Functions
+/-
+  This file serves mainly for educational purposes to demonstrate how 
+  StateM is differentiable monad. For general case look at StateT.
+ -/ 
 
-import SciLean.Core.Monad.VecMonad
+import SciLean.Core.Monad.FwdDiff.Basic
 
 set_option synthInstance.maxSize 2048
-set_option synthInstance.maxHeartbeats 100000
+-- set_option synthInstance.maxHeartbeats 100000
 
 namespace SciLean
-
-@[addPush]
-theorem add_push_lin {X Y} [Vec X] [Vec Y] (f : X → Y) [IsLin f] (x x' : X)
-  : f x + f x' = f (x + x') := sorry
-
-@[addPull]
-theorem add_pull_differential {X Y} [Vec X] [Vec Y] (f : X → Y) [IsSmooth f] (x dx dx' : X)
-  : δ f x (dx + dx') = δ f x dx + δ f x dx' := sorry
-
-@[addPull]
-theorem add_pull_prod_fst {X Y} [Add X] [Add Y] (xy xy' : X×Y)
-  : (xy + xy').1 = xy.1 + xy'.1 := sorry
-
-@[addPull]
-theorem add_pull_prod_snd {X Y} [Add X] [Add Y] (xy xy' : X×Y)
-  : (xy + xy').2 = xy.2 + xy'.2 := sorry
 
 noncomputable
 instance {σ} [Vec σ] : FwdDiffMonad (StateM σ) where
   IsSmoothM mx := IsSmooth (λ s => mx s)
   
+  ---
+
+  pure_is_smooth := by 
+    simp[pure,StateT.pure,StateM,StateT,Id]; infer_instance done
+  pure_is_smoothM x := by 
+    simp[pure,StateT.pure,StateM,StateT,Id]; infer_instance done
+
+  bind_is_smooth f hf₁ mhf₂ g hg₁ mhg₂ := by 
+    simp[compM,bind,StateT.bind,pure,StateT.pure,StateM,StateT,Id] at f hf₁ mhf₂ g hg₁ mhg₂ ⊢
+    have hg₂ : ∀ x, IsSmooth (g x) := λ x => (mhg₂ x)
+    have hf₂ : ∀ y, IsSmooth (f y) := λ y => (mhf₂ y)
+    infer_instance done
+  bind_is_smoothM f hf₁ mhf₂ mx hx := by 
+    simp[compM,bind,StateT.bind,pure,StateT.pure,StateM,StateT,Id,VecMonad] at f hf₁ mhf₂ mx hx ⊢
+    have hf₂ : ∀ y, IsSmooth (f y) := λ y => (mhf₂ y)
+
+    -- For some reason these instances fail to be infered automatically 
+    have hx' : IsSmooth λ s => (mx s) := hx
+    have hx₁ : IsSmooth λ s => (mx s).1 := by apply comp.arg_x.isSmooth
+    have hx₂ : IsSmooth λ s => (mx s).2 := by apply comp.arg_x.isSmooth
+
+    infer_instance done
+
+  diag_is_smooth f hf₁ mhf₂ g hg₁ mhg₂ := by
+    simp[compM,bind,StateT.bind,pure,StateT.pure,StateM,StateT,Id] at f hf₁ mhf₂ g hg₁ mhg₂ ⊢
+    have hg₂ : ∀ x, IsSmooth (g x) := λ x => (mhg₂ x)
+    have hf₂ : ∀ y, IsSmooth (f y) := λ y => (mhf₂ y)
+    infer_instance done
+
+  diag_is_smoothM mx hx my hy := by
+    simp[compM,bind,StateT.bind,pure,StateT.pure,StateM,StateT,Id] at mx hx my hy ⊢
+
+    -- For some reason these instances fail to be infered automatically 
+    have hx' : IsSmooth λ s => (mx s) := hx
+    have hx₁ : IsSmooth λ s => (mx s).1 := by apply comp.arg_x.isSmooth
+    have hx₂ : IsSmooth λ s => (mx s).2 := by apply comp.arg_x.isSmooth
+    have hy' : IsSmooth λ s => (my s) := hy
+    have hy₁ : IsSmooth λ s => (my s).1 := by apply comp.arg_x.isSmooth
+    have hy₂ : IsSmooth λ s => (my s).2 := by apply comp.arg_x.isSmooth
+
+    infer_instance done
+  
+  ---
+
   fwdDiffM f := λ x s => 
      let ((y,s), df) := fwdDiff (λ (x,s) => f x s) (x,s)
      ((y, λ dx ds => df (dx,ds)), s)
@@ -34,26 +65,33 @@ instance {σ} [Vec σ] : FwdDiffMonad (StateM σ) where
   fwdDiffM_id := by simp[pure,StateT.pure,StateM,StateT,Id,prod_add_elemwise,idFDM,idM]
 
   fwdDiffM_comp f hf₁ mhf₂ g hg₁ mhg₂ := by
-    simp[fwdDiff,compM,compFDM,pureZero, pure,StateT.pure,bind,StateT.bind,StateT,StateM,Id,prod_add_elemwise,uncurryFDM,fmaplrFDM] at f hf₁ mhf₂ g hg₁ mhg₂ ⊢
+    simp[fwdDiff,compM,compFDM,pure,StateT.pure,bind,StateT.bind,StateT,StateM,Id,prod_add_elemwise,fmaplrFDM] at f hf₁ mhf₂ g hg₁ mhg₂ ⊢
     have hg₂ : ∀ x, IsSmooth (g x) := λ x => (mhg₂ x)
     have hf₂ : ∀ y, IsSmooth (f y) := λ y => (mhf₂ y)
     funext x s; simp
     done
 
-  mapFDM Tf := λ x s => 
-    let (y,df) := Tf x
-    ((y, λ dx ds => (df dx, ds)), s)
+  ---
 
-  mapFDM_id := by simp[pure,StateT.pure,idFD,idFDM]
+  mapFDM_id := by simp[pure,StateT.pure,idFD,idFDM,mapFDM]
 
   mapFDM_comp Tf Tg := by 
-    simp[bind,StateT.bind,pure,StateT.pure,idFD,idFDM,compFDM,compFD]
+    simp[bind,StateT.bind,pure,StateT.pure,idFD,idFDM,compFDM,compFD,mapFDM]
+
+  ---
 
   fwdDiff_fwdDiffM f _ := by 
-    simp[fwdDiff,pure,StateT.pure,StateT,StateM,Id,prod_add_elemwise,mapM]
+    simp[fwdDiff,pure,StateT.pure,StateT,StateM,Id,prod_add_elemwise,mapM,mapFDM]
 
-  fmap_fwdDiffM f hf₁ mhf₂ g hg₁ mhg₂ := by
-    simp[fwdDiff,compM,compFDM,pureZero, pure,StateT.pure,bind,StateT.bind,StateT,StateM,Id,prod_add_elemwise,uncurryFDM,fmaplrFDM] at f hf₁ mhf₂ g hg₁ mhg₂ ⊢
+  const_fwdDiffM mx hx := by
+    simp[fwdDiff,compM,compFDM,pure,StateT.pure,bind,StateT.bind,StateT,StateM,Id,prod_add_elemwise] at mx hx ⊢
+    funext y s;
+    have hx' : IsSmooth λ s => (mx s) := hx
+    simp [diff_of_comp]
+    done
+
+  diag_fwdDiffM f hf₁ mhf₂ g hg₁ mhg₂ := by
+    simp[fwdDiff,compM,compFDM,pure,StateT.pure,bind,StateT.bind,StateT,StateM,Id,prod_add_elemwise,fmaplrFDM] at f hf₁ mhf₂ g hg₁ mhg₂ ⊢
     have hg₂ : ∀ x, IsSmooth (g x) := λ x => (mhg₂ x)
     have hf₂ : ∀ y, IsSmooth (f y) := λ y => (mhf₂ y)
     funext x s; simp[prod_add_elemwise]
