SciLean/Core/Monad/FwdDiff/StateT.lean
@@ -1,0 +1,105 @@
+import SciLean.Core.Monad.FwdDiff.IsSmoothM
+import SciLean.Core.Monad.FwdDiff.Simp
+
+set_option synthInstance.maxSize 2048
+-- set_option synthInstance.maxHeartbeats 100000
+
+namespace SciLean
+
+noncomputable
+instance {σ} [Vec σ] {m} [FwdDiffMonad m] : FwdDiffMonad (StateT σ m) where
+  IsSmoothM mx := IsSmooth (λ s => mx s) ∧ ∀ s, SciLean.IsSmoothM (mx s)
+  
+  ---
+
+  pure_is_smooth := by 
+    simp[pure,StateT.pure,StateM,StateT,Id]; infer_instance done
+  pure_is_smoothM x := by 
+    simp[pure,StateT.pure,StateM,StateT,Id]; constructor; infer_instance; infer_instance done
+
+  bind_is_smooth f hf₁ mhf₂ g hg₁ mhg₂ := by 
+    simp[compM,bind,StateT.bind,pure,StateT.pure,StateM,StateT,Id] at f hf₁ mhf₂ g hg₁ mhg₂ ⊢
+    have hg₂ : ∀ x, IsSmooth (g x) := λ x => (mhg₂ x).1
+    have hg₃ : ∀ x s, IsSmoothM (g x s) := λ x => (mhg₂ x).2
+    have hf₂ : ∀ y, IsSmooth (f y) := λ y => (mhf₂ y).1
+    have hf₃ : ∀ x s, IsSmoothM (f x s) := λ x => (mhf₂ x).2
+    infer_instance done
+  bind_is_smoothM f hf₁ mhf₂ mx hx := by 
+    simp[compM,bind,StateT.bind,pure,StateT.pure,StateM,StateT,Id,VecMonad] at f hf₁ mhf₂ mx hx ⊢
+    have hf₂ : ∀ y, IsSmooth (f y) := λ y => (mhf₂ y).1
+    have hf₃ : ∀ x s, IsSmoothM (f x s) := λ x => (mhf₂ x).2
+
+    -- For some reason these instances fail to be infered automatically 
+    have hx1 : IsSmooth λ s => (mx s) := hx.1
+    have hx2 : ∀ s, IsSmoothM (mx s) := hx.2
+
+    constructor; infer_instance; infer_instance done
+
+  diag_is_smooth f hf₁ mhf₂ g hg₁ mhg₂ := by
+    simp[compM,bind,StateT.bind,pure,StateT.pure,StateM,StateT,Id] at f hf₁ mhf₂ g hg₁ mhg₂ ⊢
+    have hg₂ : ∀ x, IsSmooth (g x) := λ x => (mhg₂ x).1
+    have hg₃ : ∀ x s, IsSmoothM (g x s) := λ x => (mhg₂ x).2
+    have hf₂ : ∀ y, IsSmooth (f y) := λ y => (mhf₂ y).1
+    have hf₃ : ∀ x s, IsSmoothM (f x s) := λ x => (mhf₂ x).2
+    infer_instance done
+
+  diag_is_smoothM mx hx my hy := by
+    simp[compM,bind,StateT.bind,pure,StateT.pure,StateM,StateT,Id] at mx hx my hy ⊢
+
+    -- For some reason these instances fail to be infered automatically 
+    have hx1 : IsSmooth λ s => (mx s) := hx.1
+    have hx2 : ∀ s, IsSmoothM (mx s) := hx.2
+    have hy1 : IsSmooth λ s => (my s) := hy.1
+    have hy2 : ∀ s, IsSmoothM (my s) := hy.2
+
+    constructor; infer_instance; infer_instance done
+  
+  ---
+
+  fwdDiffM f := λ x s => do
+     let ((y,s),df) ← fwdDiffM (λ (x,s) => f x s) (x,s)
+     pure ((y, λ dx ds => df (dx,ds)), s)
+
+  fwdDiffM_id := by simp[pure,StateT.pure,StateM,StateT,Id,prod_add_elemwise,idFDM,idM]
+
+  fwdDiffM_comp f hf₁ mhf₂ g hg₁ mhg₂ := by
+    simp[fwdDiff,compM,compFDM,pure,StateT.pure,bind,StateT.bind,StateT,StateM,Id,prod_add_elemwise,fmaplrFDM,appFDM] at f hf₁ mhf₂ g hg₁ mhg₂ ⊢
+    have hg₂ : ∀ x, IsSmooth (g x) := λ x => (mhg₂ x).1
+    have hg₃ : ∀ x s, IsSmoothM (g x s) := λ x => (mhg₂ x).2
+    have hf₂ : ∀ y, IsSmooth (f y) := λ y => (mhf₂ y).1
+    have hf₃ : ∀ x s, IsSmoothM (f x s) := λ x => (mhf₂ x).2
+    funext x s; simp[appFDM]
+    done
+
+  ---
+
+  mapFDM_id := by simp[pure,StateT.pure,idFD,idFDM,mapFDM]
+
+  mapFDM_comp Tf Tg := by
+    simp[bind,StateT.bind,pure,StateT.pure,idFD,idFDM,compFDM,compFD,mapFDM]
+
+  ---
+
+  fwdDiff_fwdDiffM f _ := by 
+    simp[fwdDiff,pure,StateT.pure,StateT,StateM,Id,prod_add_elemwise,mapM]
+    funext dx ds; simp[mapFDM,pure,StateT.pure]
+    done
+
+  const_fwdDiffM mx hx := by
+    simp[fwdDiff,compM,compFDM,pure,StateT.pure,bind,StateT.bind,StateT,StateM,Id,prod_add_elemwise] at mx hx ⊢
+    funext y s;
+    have hx1 : IsSmooth λ s => (mx s) := hx.1
+    have hx2 : ∀ s, IsSmoothM (mx s) := hx.2
+    simp [diff_of_comp,mapFDM,appFDM]
+    done
+
+  diag_fwdDiffM f hf₁ mhf₂ g hg₁ mhg₂ := by
+    simp[fwdDiff,compM,compFDM,pure,StateT.pure,bind,StateT.bind,StateT,StateM,Id,prod_add_elemwise,fmaplrFDM] at f hf₁ mhf₂ g hg₁ mhg₂ ⊢
+    have hg₂ : ∀ x, IsSmooth (g x) := λ x => (mhg₂ x).1
+    have hg₃ : ∀ x s, IsSmoothM (g x s) := λ x => (mhg₂ x).2
+    have hf₂ : ∀ y, IsSmooth (f y) := λ y => (mhf₂ y).1
+    have hf₃ : ∀ x s, IsSmoothM (f x s) := λ x => (mhf₂ x).2
+    funext x s; 
+    -- This is problematic for some reason, looks like a bug in simp
+    -- simp[idFDM, fmaplrFDM, appFDM, mapFDM]
+    sorry
